store/client_proofs/create.v
@@ -34,14 +34,14 @@ Lemma wp_client_create E c cs t1 t2 :
   store_ctx N -∗
   public t1 -∗
   public t2 -∗
-  {{{ client cs }}}
+  {{{ client cs ∗ rem_free_at cs {[t1]} }}}
     Client.create N c (repr cs) t1 t2 @ E
   {{{ (b : bool), RET #b;
       client cs ∗
-      if b then rem_mapsto cs t1 t2 else True }}}.
+      rem_mapsto cs t1 t2 }}}.
 Proof.
 iIntros "% #chan_c (_ & _ & _ & _ & _ & #? & #? & _)
-         #p_t1 #p_t2' !> %Φ client post".
+         #p_t1 #p_t2' !> %Φ [client free] post".
 iDestruct "client" as "(%n & #handshake & #key & #minted & ts & client)".
 rewrite /Client.create. wp_pures.
 wp_bind (Client.get_timestamp _).
@@ -52,7 +52,7 @@ iApply wp_client_get_session_key => //.
 iIntros "!> _". wp_pures.
 wp_list. wp_bind (tint _). iApply wp_tint. wp_list. wp_term_of_list. wp_pures.
 wp_tsenc. wp_pures.
-iMod (DB.create_client t1 t2 with "client")
+iMod (DB.create_client t1 t2 with "client free")
   as "(#create & client & up)".
 wp_bind (send _ _). iApply wp_send => //.
 { iApply public_TEncIS => //.
@@ -80,37 +80,10 @@ subst v'.
 wp_bind (Client.incr_timestamp _).
 iApply (wp_client_incr_timestamp with "ts").
 iIntros "!> ts".
-iDestruct (public_TEncE with "p_m [//]") as "{p_m} [[pub p_m]|p_m]".
-- wp_pures. wp_bind (tint _). iApply wp_tint. wp_pures.
-  iPoseProof ("key" with "pub") as ">%not_ok".
-  wp_bind (eq_term _ _). iApply wp_eq_term. wp_pures.
-  iModIntro. iRight. iExists _. iSplit => //.
-  iApply "post".
-  iPoseProof (DB.create_client_fake t1 t2 with "client") as "#fake".
-  iSplitL => //; last first.
-  { rewrite /rem_mapsto (bool_decide_eq_false_2 _ not_ok).
-    by case: bool_decide. }
-  iExists (S n). iFrame. by eauto.
-- iDestruct "p_m" as "(#p_m & _)".
-  wp_pures. wp_bind (tint _). iApply wp_tint. wp_pures.
-  iDestruct "p_m" as "(%n' & %t1' & %t2' & %b' & %si & %γ' & %e & %e_key &
-                       sessR & free)".
-  case/Spec.of_list_inj: e => en <- _ ->.
-  have {en} <- : n = n' by lia.
-  wp_bind (eq_term _ _).
-  iApply (wp_wand _ _ _ (λ v, ⌜v = #b'⌝)%I).
-  { iApply wp_eq_term. iPureIntro. by case: b'. }
-  iIntros "% ->". wp_pures. iModIntro. iRight. iExists #b'.
-  iSplit => //. iApply "post".
-  iPoseProof (DB.create_client_fake t1 t2 with "client") as "#fake".
-  iSplitL "client ts".
-  + iExists (S n). iFrame. by eauto.
-  + rewrite /rem_mapsto. case: b' => //.
-    case: bool_decide_reflect => // ok.
-    iPoseProof (session_agree with "sessR handshake") as "->" => //.
-    iDestruct ("free" with "[//] [//]") as "{free} (%γ'' & sessI' & free)".
-    iPoseProof (session_agree_name with "sessI' handshake") as "(_ & ->)" => //.
-    by iApply "up".
+wp_pures. wp_bind (tint _). iApply wp_tint.
+wp_bind (eq_term _ _). iApply wp_eq_term. wp_pures.
+iRight. iModIntro. iExists _. iSplit => //. iApply "post".
+iFrame. iExists (S n). iFrame. do !iSplit => //.
 Qed.
 
 End Verif.
